

AI-Miss Maham Gul

23/Nov/2025

ASSIGNMENT: 3

SP23-BDS-023

Khadija Jumani

SP23-BDS-053

Uzair Ali Zahid

■ APPLY Resolution for Inference : Problem Scenario

- 1- Either Alice^A, Bob^B, or Charlie^C was in the ^{In(x)}mansion at the ^ttime of the ^{t1}crime.
- 2- If Alice was in the mansion, then she ^{Saw(y)}saw the crime.
- 3- If Bob was in the mansion, then the ^{open}window was open.
- 4- If Charlie was in the mansion and the ^{Committed(x)}window was not open, then he committed the crime.
- 5- Alice didn't see the crime.
- 6- The window was not open.
- 7- Assumption :-
committed (c, y)

① Translate into First-Order Logic (FOL):-

- ① Disjunction statement \rightarrow It says at least one of them was there so;

$$\text{In}(a, t_1) \vee \text{In}(b, t_1) \vee \text{In}(c, t_1)$$

- ② Implication (If-then)

$$\text{In}(a) \rightarrow \text{saw}(a, y)$$

$$\text{or } \text{In}(a, x) \rightarrow \text{saw}(a, y)$$

- ③ $\text{In}(b) \rightarrow \text{open}$

$$\text{or } \text{In}(b, x) \rightarrow \text{open}$$

- ④ $\text{In}(c) \wedge \neg \text{open} \rightarrow \text{committed}(c, y)$

$$\text{or } \text{In}(c, x) \rightarrow \neg \text{open}$$

- ⑤ $\neg \text{saw}(A, y)$

- ⑥ $\neg \text{open}$

② Convert FOL into CNF (clausal form)

- Remove Implications ($P \rightarrow Q \equiv \neg P \vee Q$)

- ① $\text{In}(a, t_1) \vee \text{In}(b, t_1) \vee \text{In}(c, t_1)$
is already in the CNF form.

- ② $\neg \text{In}(a, x) \vee \text{saw}(a, y)$

- ③ $\neg \text{In}(b, x) \vee \text{open}$

$$\textcircled{4} \quad \neg (\text{In}(c) \wedge \neg \text{open}) \vee \text{committed}(c, y)$$

De-morgan's Law

$$\neg \text{In}(c) \vee \text{open} \vee \text{committed}(c, y)$$

$$\textcircled{5} \quad \neg \text{saw}(a, y); \text{ is already in CNF}$$

$$\textcircled{6} \quad \neg \text{open} \text{ (already in CNF)}$$

$$\textcircled{3} \quad \text{Apply Resolution (Refutation)} \quad \neg \text{committed}(c, y)$$

→ Add the negation of the query for refutation →

Available clauses :-

$$[\text{In}(a, y) \vee \text{In}(b, y) \vee \text{In}(c, y)] \vee [\text{In}(a, y) \vee \text{saw}(a, y)] \vee [\text{In}(b, y) \vee \text{open}] \vee [\neg \text{In}(c) \vee \text{open}] \vee \text{committed}(c, y) \vee [\neg \text{saw}(a, y)] \vee [\neg \text{open}]$$

→ Applying Resolution

$$\neg \text{In}(a, y) \vee \text{saw}(a, y)$$

$$\underline{\neg \text{saw}(a, y)}$$

$$\neg \text{In}(a, y) \quad \text{---} \textcircled{1}$$

$$\neg \text{In}(c) \vee \text{open} \vee \text{committed}(c, y)$$

$$\underline{\neg \text{open}}$$

$$\neg \text{In}(c) \vee \text{committed}(c, y) \quad \text{---} \textcircled{2}$$

From eq. ① and ②

$$\text{In}(a, y) \vee \text{In}(b, y) \vee \text{In}(c, y)$$

$$\text{committed}(c, y) \vee \neg \text{In}(a, y) \vee \neg \text{In}(c, y)$$

$\text{committed}(c, y) \vee \text{In}(b, y)$ — (3)

$\neg \text{In}(b, y) \vee \text{open}$

$\text{open} \vee \text{committed}(c, y)$

$\text{committed}(c, y) \vee \text{open}$

$\neg \text{open}$

$\boxed{\text{committed}(c, y)}$

(can be used again)

So,

$\text{committed}(c, y)$ and $\neg \text{committed}(c, y)$

Contradicts.

Hence query is proved that,

Charlie committed the crime!!
